theories/approxis/examples/LR_tac.v
@@ -25,19 +25,74 @@ Module Basic.
     | _ => Control.zero (Tactic_failure (Some (fprintf "no pattern found for lrel %t" lr)))
     end.
 
-  Ltac2 mutable rel_vals (lr : constr) (* : unit *) :=
-    lazy_match! lr with
-    | @lrel_unit => eauto
-    | _ => Control.zero (Tactic_failure (Some (fprintf "Don't know how to solve lrel %t" lr)))
+  Ltac2 mutable lrintro_tacs () : (string , (constr -> constr list -> (constr -> constr list -> constr option) -> constr option)) FMap.t :=
+    FMap.empty (FSet.Tags.string_tag).
+
+  Ltac2 printst st :=
+    printf "current state is:" ;
+    List.iter (fun (s, f) => printf "%s, " s) st.
+
+  Ltac2 lr_printst () :=
+    let m := lrintro_tacs () in
+    let st := FMap.bindings m in
+    printst st.
+
+  Ltac2 rec lr_intro typ xs :=
+    printf "entering lr_intro, typ: %t" typ ;
+    FMap.fold
+      (fun name f finished =>
+         match finished with
+         | Some s => finished
+         | None =>
+             (printf "trying %s" name ;
+              f typ xs lr_intro)
+         end)
+      (lrintro_tacs ())
+      None.
+
+  Ltac2 fmt_constr_opt () opt :=
+    match opt with None => Message.of_string "None"
+              | Some s => Message.concat (Message.of_string "Some ") (Message.of_constr s)
     end.
+
+  Ltac2 Type progress := [ Progressed | Stuck ].
+
+  Ltac2 mutable rel_val_tacs () : (string , (constr -> (constr -> progress) -> progress)) FMap.t :=
+    FMap.empty (FSet.Tags.string_tag).
+
+  Ltac2 rec f_rel_vals typ :=
+    printf "entering lr_intro, typ: %t" typ ;
+    FMap.fold
+      (fun name f finished =>
+         match finished with
+         | Progressed => finished
+         | Stuck =>
+             (printf "trying %s" name ;
+              f typ f_rel_vals)
+         end)
+      (rel_val_tacs ())
+      Stuck.
+
+  Ltac2 rel_vals (lr : constr) : unit :=
+    let prog := f_rel_vals lr in
+    ().
+
+  (* Ltac2 mutable rel_vals (lr : constr) : unit :=
+       lazy_match! lr with
+       | @lrel_unit => eauto
+       (* | _ => Control.zero (Tactic_failure (Some (fprintf "Don't know how to solve lrel %t" lr))) *)
+       | _ => printf "Don't know how to solve lrel %t" lr
+       end. *)
 
   Tactic Notation "lrintro" constr(x) :=
     let f :=
       ltac2val:
         (lr xs |-
-           let pat := pattern_of_lr2
-                        (Option.get (Ltac1.to_constr lr))
-                        [(Option.get (Ltac1.to_constr xs))] in
+           let pat :=
+             (* pattern_of_lr2 *)
+             (Option.get (lr_intro
+                            (Option.get (Ltac1.to_constr lr))
+                            [(Option.get (Ltac1.to_constr xs))])) in
            Ltac1.of_constr pat) in
     lazymatch goal with
     | |- environments.envs_entails _ (lrel_car ?A _ _ -∗ _) =>
@@ -70,35 +125,132 @@ Module Basic.
         f lr
     | _ => fail "rel_vals: case not covered"
     end.
-  Ltac rel_vals := try (rel_values ; iModIntro) ; rel_vals'.
+  Ltac rel_vals := try rel_values ; try iModIntro ; repeat rel_vals'.
 
 End Basic.
 Export Basic.
 
 Ltac2 get_head_name xs := match xs with [] => '"" | x :: _ => x end.
 
+Module LR_unit.
+  Ltac2 unit_intro typ xs k :=
+    printf "entering unit_intro, typ: %t" typ ;
+    lazy_match! typ with
+    | lrel_unit =>
+        printf "found `lrel_unit`, done" ;
+        Some '"(->&->)"
+    | _ => None
+    end.
+  Ltac2 Set Basic.lrintro_tacs as prev := fun () => FMap.add "unit" unit_intro (prev ()).
+End LR_unit.
+Export LR_unit.
+
+Module LR_prod.
+  Ltac2 prod_val typ k :=
+    printf "entering prod_val, typ: %t" typ ;
+    lazy_match! typ with
+    | (lrel_car lrel_prod ?v1 ?v2) =>
+        printf "found `lrel_prod %t %t`, splitting" v1 v2 ;
+        ltac1:(iExists _,_,_,_ ; iSplit ; [eauto|iSplit ; [eauto | iSplit]]) ; Progressed
+    | (lrel_car _ (?v1 , ?v2)%V (?v3 , ?v4)%V) =>
+        printf "found `_ (%t, %t) (%t, %t)`, splitting" v1 v2 v3 v4 ;
+        ltac1:(iExists _,_,_,_ ; iSplit ; [eauto|iSplit ; [eauto | iSplit]]) ; Progressed
+    | _ => Stuck
+    end.
+  Ltac2 Set Basic.rel_val_tacs as prev := fun () => FMap.add "prod" prod_val (prev ()).
+End LR_prod.
+Export LR_prod.
+
+Module LR_int.
+  Ltac2 int_intro typ xs k :=
+    printf "entering int_intro, typ: %t" typ ;
+    lazy_match! typ with
+    | lrel_int =>
+        printf "found `lrel_int`, done" ;
+        match xs with
+        | [] => Some '"(%&->&->)"
+        | x :: _ => let s := '(append "(%" ($x ++ "&->&->)")) in
+                    Some (eval vm_compute in $s)
+        end
+    | _ => None
+    end.
+  Ltac2 Set Basic.lrintro_tacs as prev := fun () => FMap.add "int" int_intro (prev ()).
+
+  Ltac2 int_val typ k :=
+    printf "entering int_val, typ: %t" typ ;
+    lazy_match! typ with
+    | (lrel_car lrel_int ?v1 ?v2) =>
+        printf "found `lrel_int %t %t`, trying lia" v1 v2 ;
+        ltac1:(iExists _ ; iPureIntro ; (intuition lia || eauto)) ; Progressed
+    | _ => Stuck
+    end.
+  Ltac2 Set Basic.rel_val_tacs as prev := fun () => FMap.add "int" int_val (prev ()).
+End LR_int.
+Export LR_int.
+
 Module LR_option.
+  Ltac2 option_intro typ xs k :=
+    printf "entering option_intro, typ: %t" typ ;
+    lazy_match! typ with
+    | lrel_option ?a =>
+        printf "found `option %t`, continuing" a ;
+        Option.bind
+          (k a xs)
+          (fun aa =>
+             Option.bind (k 'lrel_unit [])
+               (fun u =>
+                  let s := '(append "#(%" (" " ++ "&% &[(->&->&" ++ $u ++ ") | (->&->&"++$aa++")])")) in
+                  Option.ret (eval vm_compute in $s)))
+    | _ => None
+    end.
+  Ltac2 Set Basic.lrintro_tacs as prev := fun () => FMap.add "option" option_intro (prev ()).
 
-  Ltac2 Set pattern_of_lr2 as previous :=
-    fun lr (xs : constr list) =>
-      lazy_match! lr with
-      | lrel_option ?a =>
-          let aa := previous a xs in
-          let u := previous 'lrel_unit xs in
-          let s := '(append "#(%" (" " ++ "&% &[(->&->&" ++ $u ++ ") | (->&->&"++$aa++")])")) in
-          eval vm_compute in $s
-      | _ => previous lr xs
-      end.
+  (* Ltac2 Set pattern_of_lr2 as previous :=
+       fun lr (xs : constr list) =>
+         lazy_match! lr with
+         | lrel_option ?a =>
+             let aa := previous a xs in
+             let u := previous 'lrel_unit xs in
+             let s := '(append "#(%" (" " ++ "&% &[(->&->&" ++ $u ++ ") | (->&->&"++$aa++")])")) in
+             eval vm_compute in $s
+         | _ => previous lr xs
+         end. *)
 
-  Ltac2 Set rel_vals as previous :=
-    fun lr =>
-      lazy_match! lr with
-      | (lrel_car _ (InjRV _) (InjRV _)) =>
-          ltac1:(iExists _,_ ; iRight ; iSplit ; [eauto | iSplit ; eauto])
-      | (lrel_car _ (InjLV _) (InjLV _)) =>
-          ltac1:(iExists _,_ ; iLeft ; iSplit ; [eauto | iSplit ; eauto])
-      | _ => previous lr
-      end.
+  Ltac2 option_val typ k :=
+    printf "entering option_val, typ: %t" typ ;
+    lazy_match! typ with
+    | (lrel_car _ (InjLV _) (InjLV _)) =>
+        printf "found `InjLV`, continuing left" ;
+        ltac1:(iExists _,_ ; iLeft ; iSplit ; [eauto | iSplit ; eauto]) ; Progressed
+    | (lrel_car _ (InjRV _) (InjRV _)) =>
+        printf "found `InjRV`, continuing right" ;
+        ltac1:(iExists _,_ ; iRight ; iSplit ; [eauto | iSplit ; eauto]) ; Progressed
+    | _ => Stuck
+    end.
+
+  Ltac2 Set Basic.rel_val_tacs as prev := fun () => FMap.add "option" option_val (prev ()).
 
 End LR_option.
 Export LR_option.
+
+Goal forall Σ, ⊢ ∀ v1 v2, @lrel_option Σ (@lrel_int Σ) v1 v2 -∗ ⌜v1 = v2⌝.
+  ltac1:(iIntros (?) ; iStartProof ; lrintro "").
+  1:ltac1:(done).
+  lr_printst ().
+  printf "%a" fmt_constr_opt (lr_intro '(lrel_int) ['"x"]).
+  printf "%t" (pattern_of_lr2 'lrel_int ['"x"]).
+  (* printf "%t" (pattern_of_lr2 '(lrel_option lrel_int) ['"x"]). *)
+  printf "%a" fmt_constr_opt (lr_intro '(lrel_option lrel_int) ['"x"]).
+  auto.
+Abort.
+
+Goal forall Σ, ⊢ @lrel_option Σ (@lrel_int Σ) (InjRV #(1/1/4/2)) (InjRV #(0+2)).
+  ltac1:(iIntros (?) ; iStartProof).
+  ltac1:(rel_vals).
+  ltac1:(rel_vals).
+Abort.
+
+Goal forall Σ, ⊢ @lrel_option Σ (@lrel_int Σ) (InjLV #()) (InjLV #()).
+  ltac1:(iIntros (?) ; iStartProof).
+  ltac1:(rel_vals).
+Qed.
